Duper/Selection.lean
@@ -6,29 +6,43 @@ namespace Duper
 open RuleM
 open Lean
 
-def isSelectableLit (c : MClause) (i : Nat) :=
+-- Sel function 0
+def isSelectableLit0 (c : MClause) (i : Nat) :=
   c.lits[i]!.sign == false || c.lits[i]!.rhs == mkConst ``False || c.lits[i]!.lhs == mkConst ``False
 
--- Selection function that always just selects the first negative literal
-def getSelections (c : MClause) : List Nat := Id.run do
-  -- simply select first negative literal:
+-- Sel function 1
+def isSelectableLit1 (c : MClause) (i : Nat) :=
+  c.lits[i]!.sign == false
+
+-- Sel function 2
+def isSelectableLit2 (c : MClause) (i : Nat) := false
+
+-- Selection function that always just selects the first selectable literal
+def getSelections (c : MClause) : CoreM (List Nat) := do
+  -- simply select first selectable literal:
+  let selFunction ←
+    match ← getSelFunctionM with
+    | 0 => pure isSelectableLit0
+    | 1 => pure isSelectableLit1
+    | 2 => pure isSelectableLit2
+    | _ => throwError "Invalid selFunction option"
   for i in [:c.lits.size] do
-    if isSelectableLit c i then
+    if selFunction c i then
       return [i]
   return []
 
 -- Selection function that never actually selects anything
 -- def getSelections (_ : MClause) : List Nat := []
 
-def litSelectedOrNothingSelected (c : MClause) (i : Nat) :=
-  let sel := getSelections c
+def litSelectedOrNothingSelected (c : MClause) (i : Nat) : CoreM Bool := do
+  let sel ← getSelections c
   if sel == []
-  then true
-  else sel.contains i
+  then return true
+  else return sel.contains i
 
-def litSelected (c : MClause) (i : Nat) :=
-  let sel := getSelections c
-  sel.contains i
+def litSelected (c : MClause) (i : Nat) : CoreM Bool := do
+  let sel ← getSelections c
+  return sel.contains i
 
 /-- Data type to capture whether a literal in a clause is eligible.
 If it is not eligible, we distinguish the cases where there might 
@@ -52,9 +66,15 @@ instance : ToMessageData (Eligibility) := ⟨Eligibility.format⟩
 A literal L is (strictly) eligible in C if it is selected in C or there are no selected literals
 in C and L is (strictly) maximal in C. -/
 def eligibilityNoUnificationCheck (c : MClause) (alreadyReduced := true) (i : Nat) (strict := false) : RuleM Bool := do
-  match getSelections c with
+  match ← getSelections c with
   | [] => c.isMaximalLit (← getOrder) alreadyReduced i strict
   | sel => do
+    let isSelectableLit ←
+      match ← getSelFunctionM with
+      | 0 => pure isSelectableLit0
+      | 1 => pure isSelectableLit1
+      | 2 => pure isSelectableLit2
+      | _ => throwError "Invalid selFunction option"
     let isSelected := sel.contains i
     if isSelected ∧ ¬ isSelectableLit c i then
       throwError "Literal {i} in clause {c.lits} may not be selected"
@@ -68,7 +88,7 @@ def eligibilityNoUnificationCheck (c : MClause) (alreadyReduced := true) (i : Na
     The alreadyReduced variable indicates whether c has been betaEta reduced as well as whether its mvars have been instantiated
     (alreadyReduced is only set to true if both of these things are true) -/
 def eligibilityPreUnificationCheck (c : MClause) (alreadyReduced := true) (i : Nat) : RuleM Eligibility := do
-  let sel := getSelections c
+  let sel ← getSelections c
   if (sel.contains i) then
     return Eligibility.eligible -- literal is eligible and the post unification check is not necessary
   else if (sel == []) then do
