Duper/Util/Reduction.lean
@@ -14,7 +14,7 @@ partial def preprocessFact (fact : Expr) : MetaM Expr := do
     return .continue e
   -- Reduce
   trace[Preprocessing.debug] "fact before preprocessing: {fact}"
-  let fact ← withTransparency .all <| Meta.transform fact (pre := red) (usedLetOnly := false)
+  let fact ← withTransparency .instances <| Meta.transform fact (pre := red) (usedLetOnly := false)
   trace[Preprocessing.debug] "fact after preprocessing: {fact}"
   let restoreNE (e : Expr) : MetaM TransformStep := do
     match e with
