DuperOnMathlib/DuperOnMathlib/Set.lean
@@ -1,0 +1,173 @@
+-- This file contains problems from Auto's Examples/Set.lean file and serves to attempt to debug those examples
+import Mathlib.Data.Nat.Prime
+import Mathlib.Data.Set.Lattice
+import Duper.Tactic
+
+open Set
+
+variable {α β : Type _}
+
+section
+variable (s t u : Set α)
+
+#check subset_def
+#check mem_inter_iff
+#check mem_union
+#check Set.ext
+
+set_option maxHeartbeats 50000
+
+-- If preprocessing eliminates ⊆ entirely, duper can solve easily 
+theorem test1a (h : s ⊆ t) : s ∩ u ⊆ t ∩ u := by
+  rw [subset_def]
+  rw [subset_def] at h
+  duper [mem_inter_iff, subset_def]
+
+-- If duper is forced to use subset_def itself, it times out
+theorem test1b (h : s ⊆ t) : s ∩ u ⊆ t ∩ u := by
+  duper [mem_inter_iff, subset_def]
+
+-- The above two tests indicate that duper should succeed on this test with auto's preprocessing, which
+-- coincides with what we see in Auto's Examples/Set.lean
+
+------------------------------------------------------------------------------------
+set_option selFunction 0 in
+theorem test2a : s ∩ (t ∪ u) ⊆ s ∩ t ∪ s ∩ u := by
+  rw [subset_def] -- Mimics auto's definition aware preprocessing
+  duper [mem_inter_iff, mem_union, subset_def]
+
+set_option selFunction 1 in
+theorem test2b : s ∩ (t ∪ u) ⊆ s ∩ t ∪ s ∩ u := by
+  rw [subset_def] -- Mimics auto's definition aware preprocessing
+  duper [mem_inter_iff, mem_union, subset_def]
+
+set_option selFunction 2 in
+theorem test2c : s ∩ (t ∪ u) ⊆ s ∩ t ∪ s ∩ u := by
+  rw [subset_def] -- Mimics auto's definition aware preprocessing
+  duper [mem_inter_iff, mem_union, subset_def]
+
+/-
+For this problem, duper fails to solve the example using its default selection function which takes both
+inequalities and equalities of the form `e = False` as selectable. However, if duper selects only actual
+inequalities, or no literals at all (selection functions 1 and 2 respectively), then duper can solve the
+problem
+-/
+------------------------------------------------------------------------------------
+set_option selFunction 0 in
+theorem test3a : s ∩ t ∪ s ∩ u ⊆ s ∩ (t ∪ u) := by
+  rw [subset_def]
+  duper [mem_inter_iff, mem_union, subset_def]
+
+set_option selFunction 1 in
+theorem test3b : s ∩ t ∪ s ∩ u ⊆ s ∩ (t ∪ u) := by
+  rw [subset_def]
+  duper [mem_inter_iff, mem_union, subset_def]
+
+set_option selFunction 2 in
+theorem test3c : s ∩ t ∪ s ∩ u ⊆ s ∩ (t ∪ u) := by
+  rw [subset_def]
+  duper [mem_inter_iff, mem_union, subset_def]
+
+/-
+For this problem, duper fails to solve the example using its default selection function which takes both
+inequalities and equalities of the form `e = False` as selectable. However, if duper selects only actual
+inequalities, or no literals at all (selection functions 1 and 2 respectively), then duper can solve the
+problem
+-/
+------------------------------------------------------------------------------------
+#check mem_diff
+
+set_option selFunction 0 in
+theorem test4a : (s \ t) \ u ⊆ s \ (t ∪ u) := by
+  rw [subset_def]
+  duper [mem_diff, mem_union, subset_def]
+
+set_option selFunction 1 in
+theorem test4b : (s \ t) \ u ⊆ s \ (t ∪ u) := by
+  rw [subset_def]
+  duper [mem_diff, mem_union, subset_def]
+
+set_option selFunction 2 in
+theorem test4c : (s \ t) \ u ⊆ s \ (t ∪ u) := by
+  rw [subset_def]
+  duper [mem_diff, mem_union, subset_def]
+
+/-
+Duper is able to solve this problem regardless of selection function, but this does NOT coincide with what
+we see in Auto's Examples/Set.lean. There, auto seems to not be able to solve this problem
+-/
+------------------------------------------------------------------------------------
+#check Set.ext
+-- This is not an example taken from Auto.lean but serves to showcase that Duper can explode if given Set.ext
+set_option trace.Timeout.debug true in
+set_option trace.Timeout.debug.fullActiveSet true in
+theorem test5a : False := by
+  duper [Set.ext] -- Duper times out without saturating
+
+set_option includeHoistRules false in
+set_option trace.Saturate.debug true in
+theorem test5b : False := by
+  duper [Set.ext] -- Duper still doesn't saturate even when hoist rules are removed
+
+set_option firstOrderUnifierGenerator true in
+set_option trace.Saturate.debug true in
+theorem test5c : False := by
+  duper [Set.ext] -- Duper saturates reasonably quickly if the first order unifier generator is used
+
+/-
+I don't know that any of the above behavior constitutes a bug per se, but it does pose an issue given
+that we want Duper to be able to reasonably handle problems that may require lemmas like Set.ext
+-/
+------------------------------------------------------------------------------------
+set_option selFunction 0 in
+theorem test6a : s ∩ t = t ∩ s := by
+  duper [Set.ext, mem_inter_iff]
+
+set_option selFunction 1 in
+theorem test6b : s ∩ t = t ∩ s := by
+  duper [Set.ext, mem_inter_iff]
+
+set_option selFunction 2 in
+theorem test6c : s ∩ t = t ∩ s := by
+  duper [Set.ext, mem_inter_iff]
+
+set_option firstOrderUnifierGenerator true in
+theorem test6d : s ∩ t = t ∩ s := by
+  duper [Set.ext, mem_inter_iff]
+
+/-
+Duper can't get this no matter how I configure the options, despite it being so simple, but in Duper's
+defense, Zipperposition took 6 seconds to get this, so this is maybe just a lot harder than we might think
+-/
+----------------------------------------------------------------------
+set_option selFunction 0 in
+theorem test7a : s ∩ (s ∪ t) = s := by
+  duper [Set.ext, mem_union, mem_inter_iff]
+
+set_option selFunction 1 in
+theorem test7b : s ∩ (s ∪ t) = s := by
+  duper [Set.ext, mem_union, mem_inter_iff]
+
+set_option selFunction 2 in
+theorem test7c : s ∩ (s ∪ t) = s := by
+  duper [Set.ext, mem_union, mem_inter_iff]
+
+set_option firstOrderUnifierGenerator true in
+set_option trace.Timeout.debug true in
+set_option trace.Timeout.debug.fullActiveSet true in
+set_option enableSuperpositionWatchClauses true in
+set_option superpositionWatchClause1 13 in
+set_option superpositionWatchClause2 32 in
+set_option trace.Rule.superposition true in
+theorem test7d : s ∩ (s ∪ t) = s := by
+  duper [Set.ext, mem_union, mem_inter_iff]
+
+/-
+Zipperposition is able to solve this problem quickly, but Duper doesn't seem to be able to solve this
+problem under any configuration of options. I'm still in the process of investigating why this is the
+case.
+-/
+
+-- There are more problems in Auto's Examples/Set.lean file, but I haven't closely examined/moved them here yet
+
+end
